theories/Prelude/PreludeMath.v
@@ -534,6 +534,10 @@ Module Ensembles.
       pose proof (proj1 (X_repr_isFilterReprOf_X (exist _ z phi_z)) z_in_X) as z_in_X_repr...
   Qed.
 
+  Definition fromSequence {I : Type} {A : Type} (x_i : I -> A) : ensemble A :=
+    fun x : A => exists i : I, x = x_i i
+  .
+
 (** "Ensemble Tactics" *)
 
   Ltac ensemble_rewrite := autorewrite with ensemble_hints.
